\uuid{tgl8}
\exo7id{2272}
\auteur{barraud}
\datecreate{2008-04-24}
\isIndication{false}
\isCorrection{true}
\chapitre{Polynôme}
\sousChapitre{Polynôme}

\contenu{
\texte{
Trouver le $\pgcd(f,g)$ dans $\Zz_2[x]$ 
et sa repr\'esentation lin\'eaire 
$fu+gv$ o\`u $d, u,v\in \Zz_2[x]$ :
}
\begin{enumerate}
    \item \question{$$ f=x^5+x^4+1,\qquad g=x^4+x^2+1;
$$}
    \item \question{$$\quad f=x^5+x^3+x+1,\qquad g=x^4+1.
$$}
\reponse{
Utiliser l'algorithme d'Euclide. (on travaille dans $\Zz/2\Zz$).
  \begin{align*}
    x^{5}+x^{4}+1&=(x^{4}+x^{2}+1)(x+1)+x^{3}+x^{2}+x\\
    x^{4}+x^{2}+1&=(x^{3}+x^{2}+x)(x+1)+x^{2}+x+1\\
    x^{3}+x^{2}+x&=(x^{2}+x+1)x+0\\
  \end{align*}
  Donc $\pgcd(x^{5}+x^{4}+1,x^{4}+x^{2}+1)=x^{2}+x+1$, et
  \begin{align*}
    x^{2}+x+1&=(x^{4}+x^{2}+1)+(x^{3}+x^{2}+x)(x+1)\\
    &=(x^{4}+x^{2}+1)+\big((x^{5}+x^{4}+1)+(x^{4}+x^{2}+1)(x+1)\big)(x+1)\\
    &=(x^{4}+x^{2}+1)(1+(x+1)^{2})+(x^{5}+x^{4}+1)(x+1)\\
    &=(x^{4}+x^{2}+1)(x^{2})+(x^{5}+x^{4}+1)(x+1)\\
  \end{align*}

  \smallskip
  De même, $\pgcd(x^{5}+x^{3}+x+1,x^{4}+1)=x^{3}+1$ et
  $x^{3}+1=(x^{5}+x^{3}+x+1)+(x^{4}+1)x$.
}
\end{enumerate}
}
