\uuid{RWnh}
\exo7id{5695}
\auteur{rouget}
\organisation{exo7}
\datecreate{2010-10-16}
\isIndication{false}
\isCorrection{true}
\chapitre{Série numérique}
\sousChapitre{Autre}

\contenu{
\texte{
Trouver un développement limité à l'ordre $4$ quand $n$ tend vers l'infini de $\left(e-\sum_{k=0}^{n}\frac{1}{k!}\right)\times(n+1)!$.
}
\reponse{
Pour $n\in\Nn$, posons $u_n= (n+1)!\left(e-\sum_{k=0}^{n}\frac{1}{k!}\right)$. Soit $n\in\Nn$.

\begin{align*}\ensuremath
u_n&=\sum_{k=n+1}^{+\infty}\frac{(n+1)!}{k!}\\
 &=1+\frac{1}{n+2}+\frac{1}{(n+2)(n+3)}+\frac{1}{(n+2)(n+3)(n+4)}+\frac{1}{(n+2)(n+3)(n+4)(n+5)}+\sum_{k=n+6}^{+\infty}\frac{1}{(n+2)(n+3)\ldots k}
\end{align*}
	

On a $0 <\sum_{k=n+6}^{+\infty}\frac{1}{(n+2)(n+3)\ldots k}=\sum_{k=n+1}^{+\infty}\frac{1}{(n+2)^{k-(n+1)}}=\frac{1}{(n+2)^5}\frac{1}{1-\frac{1}{n+2}}=\frac{1}{(n+2)^4(n+1)}\leqslant\frac{1}{n^5}$. On en déduit que $\sum_{k=n+6}^{+\infty}\frac{1}{(n+2)(n+3)\ldots k}\underset{n\rightarrow+\infty}{=}o\left(\frac{1}{n^4}\right)$. Donc

\begin{align*}\ensuremath
u_n&\underset{n\rightarrow+\infty}{=}1+\frac{1}{n+2}+\frac{1}{(n+2)(n+3)}+\frac{1}{(n+2)(n+3)(n+4)}+\frac{1}{(n+2)(n+3)(n+4)(n+5)}+o\left(\frac{1}{n^4}\right)\\
 &\underset{n\rightarrow+\infty}{=}1+\frac{1}{n}\left(1+\frac{2}{n}\right)^{-1}+\frac{1}{n^2}\left(1+\frac{2}{n}\right)^{-1}\left(1+\frac{3}{n}\right)^{-1}+\frac{1}{n^3}\left(1+\frac{2}{n}\right)^{-1}\left(1+\frac{3}{n}\right)^{-1}\left(1+\frac{4}{n}\right)^{-1}+\frac{1}{n^4}+o\left(\frac{1}{n^4}\right)\\
  &\underset{n\rightarrow+\infty}{=}1+\frac{1}{n}\left(1-\frac{2}{n}+\frac{4}{n^2}-\frac{8}{n^3}\right)+\frac{1}{n^2}\left(1-\frac{2}{n}+\frac{4}{n^2}\right)\left(1-\frac{3}{n}+\frac{9}{n^2}\right)+\frac{1}{n^3}\left(1-\frac{2}{n}\right)\left(1-\frac{3}{n}\right)\left(1-\frac{4}{n}\right)\\
  &\;+\frac{1}{n^4}+o\left(\frac{1}{n^4}\right)\\
  &\underset{n\rightarrow+\infty}{=}1+\frac{1}{n}\left(1-\frac{2}{n}+\frac{4}{n^2}-\frac{8}{n^3}\right)+\frac{1}{n^2}\left(1-\frac{5}{n}+\frac{19}{n^2}\right)+\frac{1}{n^3}\left(1-\frac{9}{n}\right)+\frac{1}{n^4}+o\left(\frac{1}{n^4}\right)\\
  &\underset{n\rightarrow+\infty}{=}1+\frac{1}{n}-\frac{1}{n^2}+\frac{3}{n^4}+o\left(\frac{1}{n^4}\right).
\end{align*}

Finalement

\begin{center}
\shadowbox{
$(n+1)!\left(e-\sum_{k=0}^{n}\frac{1}{k!}\right)\underset{n\rightarrow+\infty}{=}1+\frac{1}{n}-\frac{1}{n^2}+\frac{3}{n^4}+o\left(\frac{1}{n^4}\right)$.
}
\end{center}
}
}
