\uuid{wZNn}
\exo7id{3968}
\auteur{quercia}
\organisation{exo7}
\datecreate{2010-03-11}
\isIndication{false}
\isCorrection{true}
\chapitre{Dérivabilité des fonctions réelles}
\sousChapitre{Autre}

\contenu{
\texte{
Calculer la dérivée $n^{\text{ème}}$ de $x \mapsto x^n(1-x)^n$.
En déduire la valeur de $\sum_{k=0}^n \bigl(C_n^k\bigr)^2$.
}
\reponse{
$\frac{d^n}{d x^n}\bigl(x^n(1-x)^n\bigr) =
         \sum_{k=0}^n n!\,\bigl(C_n^k\bigr)^2 (-1)^{n-k} x^{n-k}(1-x)^k$.
         \par
         coefficient de $x^n = (-1)^n n!\, \sum_{k=0}^n \bigl(C_n^k\bigr)^2
                             = (-1)^n A_{2n}^n$.
}
}
