\uuid{wmWw}
\exo7id{5733}
\auteur{rouget}
\datecreate{2010-10-16}
\isIndication{false}
\isCorrection{true}
\chapitre{Suite et série de fonctions}
\sousChapitre{Convergence simple, uniforme, normale}

\contenu{
\texte{
Montrer que pour tout réel $a > 0$, $\int_{0}^{1}\frac{1}{1+x^a}\;dx=\sum_{n=0}^{+\infty}\frac{(-1)^n}{1+na}$.
}
\reponse{
Soit $n\in\Nn$.

\begin{center}
$\sum_{k=0}^{n}\frac{(-1)^k}{1+ka}=\sum_{k=0}^{n}(-1)^k\int_{0}^{1}t^{ka}\;dt=\int_{0}^{1}\left(\sum_{k=0}^{n}(-t^a)^k\right)\;dt=\int_{0}^{1}\frac{1}{1+t^a}\;dt+(-1)^n\int_{0}^{1}\frac{t^{(n+1)a}}{1+t^a}\;dt$,
\end{center}

avec $\left|(-1)^n\int_{0}^{1}\frac{t^{(n+1)a}}{1+t^a}\;dt\right|\leqslant\int_{0}^{1}t^{(n+1)a}\;dt=\frac{1}{1+(n+1)a}$. Par suite, $\lim_{n \rightarrow +\infty}(-1)^n\int_{0}^{1}\frac{t^{(n+1)a}}{1+t^a}\;dt=0$. On en déduit que la série de terme général $\frac{(-1)^k}{1+ka}$, $k\geqslant 0$, converge et que

\begin{center}
\shadowbox{
$\sum_{k=0}^{+\infty}\frac{(-1)^k}{1+ka}=\int_{0}^{1}\frac{1}{1+t^a}\;dt$.
}
\end{center}
}
}
