\uuid{b1ht}
\exo7id{4065}
\auteur{quercia}
\organisation{exo7}
\datecreate{2010-03-11}
\isIndication{false}
\isCorrection{true}
\chapitre{Equation différentielle}
\sousChapitre{Equations différentielles linéaires}

\contenu{
\texte{
Résoudre le système différentiel suivant :
$\begin{cases}(t^2+1)x' = tx + y + 2t^2-1\cr
        (t^2+1)y' = x - ty + 3t.\cr\end{cases}$
}
\reponse{
$y = (t^2+1)x' -tx -2t^2+1  \Rightarrow  (t^2+1)x'' + 2tx' -2x = 6t$.\par
Résolution par DSE $ \Rightarrow  x = a(1+t\arctan t) + bt + t\ln(1+t^2)$,
                        $y = a\arctan t + b + 1 + \ln(1+t^2)$.
}
}
