\uuid{Dzp8}
\exo7id{4317}
\auteur{quercia}
\organisation{exo7}
\datecreate{2010-03-12}
\isIndication{false}
\isCorrection{true}
\chapitre{Intégration}
\sousChapitre{Intégrale de Riemann dépendant d'un paramètre}

\contenu{
\texte{
\'Etablir la convergence et calculer la somme de
    $\sum_{n=1}^\infty (-1)^n \int_0^{+\infty} \frac{dt}{(1+t^3)^n}$.
}
\reponse{
$\sum_{n=1}^N (-1)^n \int_0^{+\infty} \frac{dt}{(1+t^3)^n} =
	       \int_0^{+\infty}\Bigl(1-\frac{(-1)^N}{(1+t^3)^N}\Bigr)\frac{dt}{2+t^3}
	      \to  \int_0^{+\infty}\frac{dt}{2+t^3} =
	      \frac{\pi2^{5/3}}{3\sqrt3}$ lorsque $N\to\infty$.
}
}
