\uuid{7vwz}
\exo7id{4033}
\auteur{quercia}
\organisation{exo7}
\datecreate{2010-03-11}
\isIndication{false}
\isCorrection{true}
\chapitre{Développement limité}
\sousChapitre{Autre}

\contenu{
\texte{
Développer de deux manières $(1-e^x)^n$ en $0$ à l'ordre $n+2$.

En déduire $\sum_{k=0}^n(-1)^kC_n^kk^p$ pour $p = 0,1,\dots,n+2$.
}
\reponse{
$(1-e^x)^n = \sum_{k=0}^n(-1)^kC_n^ke^{kx}
 = \sum_{p=0}^{n+2} \Bigl(\sum_{k=0}^n(-1)^kC_n^kk^p \Bigr) \frac {x^p}{p!}
   + o (x^{n+2})$,

$(1-e^x)^n = (-x)^n\left({1 + \frac {nx}2 + \frac {n(3n+1)}{24}x^2 + o  (x^2)}\right)$.
}
}
