\uuid{PvtY}
\exo7id{4714}
\auteur{quercia}
\datecreate{2010-03-16}
\isIndication{false}
\isCorrection{true}
\chapitre{Suite}
\sousChapitre{Suite définie par une relation de récurrence}

\contenu{
\texte{

}
\begin{enumerate}
    \item \question{Soient $x,y,z \ge 0$. Montrer que $x^3+y^3+z^3 - 3xyz \ge 0$
    (mettre $x+y+z$ en facteur).}
\reponse{$x^3+y^3+z^3 - 3xyz = \frac 12 (x+y+z)\bigl((x-y)^2 + (y-z)^2 + (z-x)^2\bigr)$.}
    \item \question{{\'E}tudier la convergence des suites $(a_n)$, $(b_n)$, $(c_n)$ d{\'e}finies par :
    $$0 < a_0 < b_0 < c_0,\quad \text{et}\quad
     \begin{cases}\frac 3{a_{n+1}} = \frac 1{a_n} + \frac 1{b_n} + \frac 1{c_n} \cr
            b_{n+1} = \sqrt[3]{a_nb_nc_n} \cr
            3c_{n+1} = a_n + b_n + c_n. \cr\end{cases}$$}
\reponse{$3c_{n+1} - 3b_{n+1} = a_n + b_n + c_n - 3\sqrt[3]{a_nb_nc_n} \ge 0  \Rightarrow  b_{n+1} \le c_{n+1}$.\par
    $\frac 3{a_{n+1}} - \frac 3{b_{n+1}} =
    \frac 1{a_n} + \frac 1{b_n} + \frac 1{c_n} - \frac 3{\sqrt[3]{a_nb_nc_n}}
    \ge 0  \Rightarrow  a_{n+1} \le b_{n+1}$.
    \par
    Donc $(a_n)$ cro{\^\i}t et $(c_n)$ d{\'e}cro{\^\i}t :
    $a_n \longrightarrow a$,
    $b_n \longrightarrow b$,
    $c_n \longrightarrow c$
    avec $\begin{cases} \frac 2a = \frac 1b + \frac 1c \cr b^2 = ac \cr 2c = a+b\cr\end{cases}
          \Rightarrow  a=b=c$.}
\end{enumerate}
}
