\uuid{Z1Jg}
\exo7id{4434}
\auteur{quercia}
\datecreate{2010-03-14}
\isIndication{false}
\isCorrection{true}
\chapitre{Série numérique}
\sousChapitre{Autre}

\contenu{
\texte{
On admet que $\sum_{k=1}^\infty \frac {(-1)^{k+1}}k = \ln 2$.
Montrer que la série $\sum_{k=1}^\infty \frac1{1^2 + 2^2 + \dots + k^2}$ est
convergente et calculer sa somme.
}
\reponse{
$\frac 1{1^2 + 2^2 + \dots + k^2} = \frac 6k + \frac 6{k+1}
         - \frac {24}{2k+1}
          \Rightarrow  s_n = 18 - 24\sum_{k=1}^{2n+1} \frac{(-1)^{k+1}}k
         + \frac 6{n+1} \to 18 - 24\ln 2$ lorsque $n\to\infty$.
}
}
