\uuid{b8iz}
\exo7id{2957}
\auteur{quercia}
\datecreate{2010-03-08}
\isIndication{false}
\isCorrection{true}
\chapitre{Nombres complexes}
\sousChapitre{Trigonom√©trie}

\contenu{
\texte{
Simplifier $$\sum_{k=1}^n\, \frac 1
{2^k \cos\theta \cos2\theta \cos4\theta \dots \cos2^{k-1}\theta}.$$
}
\reponse{
$S = \frac {u-u^{-1}}{u^2-u^{-2}} +
     \frac {u-u^{-1}}{u^4-u^{-4}} + \dots +
     \frac {u-u^{-1}}{u^{2^n}-u^{-2^n}}$.
\par
$\frac {u-u^{-1}}{u^2-u^{-2}} +
 \frac {u-u^{-1}}{u^4-u^{-4}} =
 \frac {u^3-u^{-3}}{u^4-u^{-4}}$.
\par
$\frac {u^3-u^{-3}}{u^4-u^{-4}} +
 \frac {u-u^{-1}}{u^8-u^{-8}} =
 \frac {u^7-u^{-7}}{u^8-u^{-8}}$
$\ldots$
\par
$ \Rightarrow  S = \frac {u^{2^n-1}-u^{-2^n+1}}{u^{2^n}-u^{-2^n}}
       = \frac {\sin\bigl((2^n-1)\theta\bigr)}{\sin(2^n\theta)}$.
}
}
