\uuid{jRsA}
\exo7id{5334}
\auteur{rouget}
\datecreate{2010-07-04}
\isIndication{false}
\isCorrection{true}
\chapitre{Polynôme, fraction rationnelle}
\sousChapitre{Autre}

\contenu{
\texte{
Déterminer deux polynômes $U$ et $V$ vérifiant $UX^n+V(1-X)^m=1$ et $\mbox{deg}(U)<m$ et $\mbox{deg}(V)<n$.
}
\reponse{
\begin{align*}\ensuremath
1&=(X+(1-X))^{n+m-1}=\sum_{k=0}^{n+m-1}C_{n+m-1}^{k}X^k(1-X)^{n+m-1-k}\\
 &=\sum_{k=0}^{n-1}C_{n+m-1}^{k}X^k(1-X)^{n+m-1-k}
+\sum_{k=n}^{n+m-1}C_{n+m-1}^{k}X^k(1-X)^{n+m-1-k}\\ 
 &=(1-X)^m\sum_{k=0}^{n-1}C_{n+m-1}^{k}X^k(1-X)^{n-1-k}+X^n\sum_{k=n}^{n+m-1}C_{n+m-1}^{k}X^{k-n}(1-X)^{n+m-1-k}
\end{align*}

Soient $U=\sum_{k=n}^{n+m-1}C_{n+m-1}^{k}X^{k-n}(1-X)^{n+m-1-k}$ et $V=\sum_{k=0}^{n-1}C_{n+m-1}^{k}X^k(1-X)^{n-1-k}$. $U$ et $V$ sont des polynômes tels que $UX^n+V(1-X)^m=1$. De plus, pour $n\leq k\leq n+m-1$, $\mbox{deg}(X^{k-n}(1-X)^{n+m-1-k})=k-n+n+m-1-k=m-1<m$ et donc $\mbox{deg}(U)<m$ et de même pour $0\leq k\leq n-1$, $\mbox{deg}(X^k(1-X)^{n-1-k})=k+n-1-k=n-1<n$ et $\mbox{deg}(V)<n$.
}
}
