\uuid{lOod}
\exo7id{170}
\auteur{cousquer}
\organisation{exo7}
\datecreate{2003-10-01}
\isIndication{false}
\isCorrection{false}
\chapitre{Logique, ensemble, raisonnement}
\sousChapitre{Récurrence}

\contenu{
\texte{

}
\begin{enumerate}
    \item \question{Démontrer par récurrence:
$$ \sum_{k=0}^n k = \frac{n(n+1)}{2} $$}
    \item \question{Calculer de deux manières différentes:
$$ \sum_{k=1}^{n+1} k^3 - \sum_{k=0}^n (k+1)^3. $$}
    \item \question{En déduire:
 $$ \sum_{k=0}^n k^2 = {1 \over 6} (2n^3+3n^2+3n). $$}
\end{enumerate}
}
